linux/pkvm/proofs/spinlock/spinlock_proof.v
@@ -382,7 +382,7 @@ Section proofs.
           iDestruct "Hcases" as "[[Hticket' %] | Htok]".
           { iExFalso. by iApply (ticket_non_duplicable with "Hticket Hticket'"). }
           iAssert (⌜owner ∈ u16⌝)%I as %[??].
-          { rewrite /ty_own_val /=. by iDestruct "Hv" as %Hv%val_of_int_in_range. }
+          { rewrite /ty_own_val /=. by iDestruct "Hv" as %Hv%val_of_Z_in_range. }
           iAssert (⌜owner < next⌝)%I as %?.
           { destruct (decide (owner < next)); first done. iExFalso.
             iDestruct (ty_size_eq with "Hv") as %?.
@@ -484,7 +484,7 @@ Section proofs.
         (* Learn that [next'] actually is [max_int u16]. *)
         iAssert ⌜next' = max_int u16⌝%I as %->.
         { iDestruct (ty_deref with "Hnext") as (w) "[_ H]". iDestruct "H" as %Hnext.
-          iPureIntro. apply val_of_int_in_range in Hnext as [??]. lia. }
+          iPureIntro. apply val_of_Z_in_range in Hnext as [??]. lia. }
         (* We perform the write and close the invariant. *)
         iDestruct (ty_aligned with "Howner") as %?.
         iDestruct (ty_deref with "Howner") as (v') "[Hl Hv]".
@@ -511,7 +511,7 @@ Section proofs.
         iAssert ⌜owner' = 0⌝%I as %->.
         { destruct (decide (owner' = 0)) => //. iExFalso.
           iDestruct (ty_deref with "Howner") as (?) "[? Hv]".
-          iDestruct "Hv" as %Howner%val_of_int_in_range. destruct Howner as [Howner ?].
+          iDestruct "Hv" as %Howner%val_of_Z_in_range. destruct Howner as [Howner ?].
           iDestruct (overlaping_ticket_ranges with "[] Htk Htr1") as "$".
           iPureIntro. exists 0. split; apply elem_of_seqZ; try done.
           split => //. rewrite /min_int /= in Howner. lia. }
@@ -558,7 +558,7 @@ Section proofs.
         iDestruct (ty_aligned with "Howner") as %?.
         iDestruct (ty_deref with "Howner") as (v') "[Hl Hv]".
         iDestruct (ty_size_eq with "Hv") as %?.
-        iDestruct "Hv" as %?%val_of_int_in_range.
+        iDestruct "Hv" as %?%val_of_Z_in_range.
         iSplitL "Hl". { iExists _. by iFrame "Hl". }
         iIntros "!> Hl".
         iMod "Hclose" as "_". iMod ("Hclose_inv" with "[Htok H● H◯ Hticket Hnext Hl Htk1 Htk2]") as "_".
@@ -568,8 +568,8 @@ Section proofs.
           iSplit. { iPureIntro. by lia. }
           iDestruct ((ty_ref (t := (owner + 1) @ int u16)) with "[] Hl []") as "$" => //.
           { iPureIntro. rewrite /i2v.
-            destruct (val_of_int (owner + 1) u16) eqn:Heq => //. exfalso.
-            assert (owner + 1 ∈ u16) as Hu16%val_of_int_is_some by (split; lia).
+            destruct (val_of_Z (owner + 1) u16) eqn:Heq => //. exfalso.
+            assert (owner + 1 ∈ u16) as Hu16%val_of_Z_is_some by (split; lia).
             destruct Hu16 as [??]. by simplify_eq. }
           iRight. iFrame "Htok". by iExists _. }
         iModIntro.
