theories/typing/optional.v
@@ -11,7 +11,7 @@ Class Optionable `{!typeG Σ} (ty : type) `{!Movable ty} (optty : type) `{!Movab
   opt_alt_sz : optty.(ty_layout) = ty.(ty_layout);
   opt_bin_op (bty beq : bool) v1 v2 σ v :
     (⊢ opt_pre v1 v2 -∗ (if bty then v1 ◁ᵥ ty else v1 ◁ᵥ optty) -∗ v2 ◁ᵥ optty -∗ state_ctx σ -∗
-        ⌜eval_bin_op (if beq then EqOp else NeOp) ot1 ot2 σ v1 v2 v ↔ val_of_int (Z_of_bool (xorb bty beq)) i32 = Some v⌝);
+        ⌜eval_bin_op (if beq then EqOp else NeOp) ot1 ot2 σ v1 v2 v ↔ val_of_Z (Z_of_bool (xorb bty beq)) i32 = Some v⌝);
 }.
 Arguments opt_pre {_ _} _ {_ _ _ _ _ _} _ _.
 
@@ -172,7 +172,7 @@ Section optional.
         iIntros (σ v) "Hctx". iDestruct "HT" as "[Hpre _]".
         iDestruct (opt_bin_op true true with "Hpre Hv1 Hv2 Hctx") as %->.
         iPureIntro. rewrite /i2v.
-        have [|v' ->] := val_of_int_is_some i32 (Z_of_bool false) => //.
+        have [|v' ->] := val_of_Z_is_some i32 (Z_of_bool false) => //.
         naive_solver.
       }
       iDestruct "HT" as "[_ [HT _]]".
@@ -182,7 +182,7 @@ Section optional.
         iIntros (σ v) "Hctx". iDestruct "HT" as "[Hpre _]".
         iDestruct (opt_bin_op false true with "Hpre Hv1 Hv2 Hctx") as %->.
         iPureIntro. rewrite /i2v.
-        have [|v' ->] := val_of_int_is_some i32 (Z_of_bool true) => //.
+        have [|v' ->] := val_of_Z_is_some i32 (Z_of_bool true) => //.
         naive_solver.
       }
       iDestruct "HT" as "[_ [_ HT]]".
@@ -199,7 +199,7 @@ Section optional.
       typed_bin_op v1 (v1 ◁ᵥ ty) v2 (v2 ◁ᵥ optty) EqOp ot1 ot2 T.
   Proof.
     iIntros "HT Hv1 Hv2". iIntros (Φ) "HΦ".
-    have [|v' Hv] := val_of_int_is_some i32 (Z_of_bool false) => //.
+    have [|v' Hv] := val_of_Z_is_some i32 (Z_of_bool false) => //.
     iApply (wp_binop_det v'). iSplit. {
       iIntros (σ v) "Hctx". iDestruct "HT" as "[Hpre _]".
       iDestruct (opt_bin_op true true with "Hpre Hv1 Hv2 Hctx") as %->.
@@ -225,7 +225,7 @@ Section optional.
         iIntros (σ v) "Hctx". iDestruct "HT" as "[Hpre _]".
         iDestruct (opt_bin_op true false with "Hpre Hv1 Hv2 Hctx") as %->.
         iPureIntro. rewrite /i2v.
-        have [|v' ->] := val_of_int_is_some i32 (Z_of_bool true) => //.
+        have [|v' ->] := val_of_Z_is_some i32 (Z_of_bool true) => //.
         naive_solver.
       }
       iDestruct "HT" as "[_ [HT _]]".
@@ -235,7 +235,7 @@ Section optional.
         iIntros (σ v) "Hctx". iDestruct "HT" as "[Hpre _]".
         iDestruct (opt_bin_op false false with "Hpre Hv1 Hv2 Hctx") as %->.
         iPureIntro. rewrite /i2v.
-        have [|v' ->] := val_of_int_is_some i32 (Z_of_bool false) => //.
+        have [|v' ->] := val_of_Z_is_some i32 (Z_of_bool false) => //.
         naive_solver.
       }
       iDestruct "HT" as "[_ [_ HT]]".
@@ -375,7 +375,7 @@ Section optionalO.
   Proof.
     unfold destruct_hint. iIntros "HT Hv1 Hv2". iIntros (Φ) "HΦ".
     destruct b.
-    - have [|v' Hv] := val_of_int_is_some i32 (Z_of_bool false) => //.
+    - have [|v' Hv] := val_of_Z_is_some i32 (Z_of_bool false) => //.
       iApply (wp_binop_det v'). iSplit. {
         iIntros (σ v) "Hctx". iDestruct "HT" as "[Hpre _]".
         iDestruct (opt_bin_op true true with "Hpre [Hv1] [Hv2] Hctx") as %->.
@@ -383,7 +383,7 @@ Section optionalO.
       }
       iDestruct ("HT" with "Hv1") as "HT".
       iApply "HΦ" => //. by rewrite /ty_own_val/=.
-    - have [|v' Hv] := val_of_int_is_some i32 (Z_of_bool true) => //.
+    - have [|v' Hv] := val_of_Z_is_some i32 (Z_of_bool true) => //.
       iApply (wp_binop_det v'). iSplit. {
         iIntros (σ v) "Hctx". iDestruct "HT" as "[Hpre _]".
         iDestruct (opt_bin_op false true with "Hpre [Hv1] [Hv2] Hctx") as %->.
@@ -405,7 +405,7 @@ Section optionalO.
   Proof.
     unfold destruct_hint. iIntros "HT Hv1 Hv2". iIntros (Φ) "HΦ".
     destruct b.
-    - have [|v' Hv] := val_of_int_is_some i32 (Z_of_bool true) => //.
+    - have [|v' Hv] := val_of_Z_is_some i32 (Z_of_bool true) => //.
       iApply (wp_binop_det v'). iSplit. {
         iIntros (σ v) "Hctx". iDestruct "HT" as "[Hpre _]".
         iDestruct (opt_bin_op true false with "Hpre [Hv1] [Hv2] Hctx") as %->.
@@ -413,7 +413,7 @@ Section optionalO.
       }
       iDestruct ("HT" with "Hv1") as "HT".
       iApply "HΦ" => //. by rewrite /ty_own_val/=.
-    - have [|v' Hv] := val_of_int_is_some i32 (Z_of_bool false) => //.
+    - have [|v' Hv] := val_of_Z_is_some i32 (Z_of_bool false) => //.
       iApply (wp_binop_det v'). iSplit. {
         iIntros (σ v) "Hctx". iDestruct "HT" as "[Hpre _]".
         iDestruct (opt_bin_op false false with "Hpre [Hv1] [Hv2] Hctx") as %->.
@@ -475,7 +475,7 @@ Section int_optional.
   Next Obligation. move => ??.  done. Qed.
   Next Obligation.
     move => ?? [] [] ????; iIntros "_" (Hv1 Hv2) "_ !%";
-    rewrite val_of_int_bool;
+    rewrite val_of_Z_bool;
     move: (Hv1) (Hv2) => /val_to_of_int? /val_to_of_int?;
     split => Hin; first [
        by simplify_eq; econstructor => //; case_bool_decide => //; lia |
